erasure/theories/EWcbvEval.v
@@ -37,11 +37,13 @@ Definition atom t :=
   | _ => false
   end.
 
-Definition isFixApp t :=
-  match fst (decompose_app t) with
-  | tFix _ _ => true
-  | _ => false
-  end.
+Definition isFixApp t := isFix (head t).
+Definition isConstructApp t := isConstruct (head t).
+
+Lemma isFixApp_mkApps f l : isFixApp (mkApps f l) = isFixApp f.
+Proof. rewrite /isFixApp head_mkApps //. Qed.
+Lemma isConstructApp_mkApps f l : isConstructApp (mkApps f l) = isConstructApp f.
+Proof. rewrite /isConstructApp head_mkApps //. Qed.
 
 Definition isStuckFix t (args : list term) :=
   match t with
@@ -58,6 +60,9 @@ Proof.
   revert f; induction l using rev_ind. simpl. intuition auto.
   simpl. intros. now rewrite mkApps_app in H.
 Qed.
+
+Definition cstr_arity (mdecl : mutual_inductive_body) (cdecl : Kernames.ident × nat) := 
+  (mdecl.(ind_npars) + cdecl.2)%nat.
 
 (* Tells if the evaluation relation should include match-prop and proj-prop reduction rules. *)
 Class WcbvFlags := { with_prop_case : bool ; with_guarded_fix : bool }.
@@ -92,10 +97,11 @@ Section Wcbv.
       eval (tLetIn na b0 b1) res
 
   (** Case *)
-  | eval_iota ind pars discr c args brs br res :
+  | eval_iota ind pars cdecl discr c args brs br res :
       eval discr (mkApps (tConstruct ind c) args) ->
-      inductive_isprop_and_pars Σ ind = Some (false, pars) ->
+      constructor_isprop_pars_decl Σ ind c = Some (false, pars, cdecl) ->
       nth_error brs c = Some br ->
+      #|args| = pars + cdecl.2 ->
       #|skipn pars args| = #|br.1| ->
       eval (iota_red pars args br) res ->
       eval (tCase (ind, pars) discr brs) res
@@ -157,10 +163,12 @@ Section Wcbv.
       eval (tConst c) res
 
   (** Proj *)
-  | eval_proj i pars arg discr args res :
+  | eval_proj i pars cdecl arg discr args a res :
       eval discr (mkApps (tConstruct i 0) args) ->
-      inductive_isprop_and_pars Σ i = Some (false, pars) ->
-      eval (List.nth (pars + arg) args tDummy) res ->
+      constructor_isprop_pars_decl Σ i 0 = Some (false, pars, cdecl) ->
+      #|args| = pars + cdecl.2 ->
+      nth_error args (pars + arg) = Some a ->
+      eval a res ->
       eval (tProj (i, pars, arg) discr) res
 
   (** Proj *)
@@ -170,10 +178,19 @@ Section Wcbv.
       inductive_isprop_and_pars Σ i = Some (true, pars) ->
       eval (tProj (i, pars, arg) discr) tBox
 
+  (** Constructor congruence: we do not allow over-applications *)
+  | eval_construct ind c mdecl idecl cdecl f args a a' : 
+    lookup_constructor Σ ind c = Some (mdecl, idecl, cdecl) ->
+    eval f (mkApps (tConstruct ind c) args) -> 
+    #|args| < cstr_arity mdecl cdecl ->
+    eval a a' ->
+    eval (tApp f a) (tApp (mkApps (tConstruct ind c) args) a')
+
+
   (** Atoms (non redex-producing heads) applied to values are values *)
   | eval_app_cong f f' a a' :
       eval f f' ->
-      ~~ (isLambda f' || (if with_guarded_fix then isFixApp f' else isFix f') || isBox f') ->
+      ~~ (isLambda f' || (if with_guarded_fix then isFixApp f' else isFix f') || isBox f' || isConstructApp f')  ->
       eval a a' ->
       eval (tApp f a) (tApp f' a')
 
@@ -203,119 +220,151 @@ Section Wcbv.
       - unapplied fixpoints and cofixpoints
    *)
 
-  Definition value_head x :=
-    isConstruct x || isCoFix x.
+   Variant value_head (nargs : nat) : term -> Type :=
+   | value_head_cstr ind c mdecl idecl cdecl :
+     lookup_constructor Σ ind c = Some (mdecl, idecl, cdecl) ->
+     nargs <= cstr_arity mdecl cdecl ->
+     value_head nargs (tConstruct ind c)
+   | value_head_cofix mfix idx : value_head nargs (tCoFix mfix idx)
+   | value_head_fix mfix idx rarg fn : 
+     cunfold_fix mfix idx = Some (rarg, fn) ->
+     (* If fixpoints are not guarded, we don't need to consider applied fixpoints 
+        as value heads*)
+     (if with_guarded_fix then nargs <= rarg else False) ->
+     value_head nargs (tFix mfix idx).
+   Derive Signature NoConfusion for value_head.
+ 
+   Inductive value : term -> Type :=
+   | value_atom t : atom t -> value t
+   | value_app_nonnil f args : value_head #|args| f -> args <> [] -> All value args -> value (mkApps f args).
+   Derive Signature for value.
 
-  Inductive value : term -> Type :=
-  | value_atom t : atom t -> value t
-  | value_app t l : value_head t -> All value l -> value (mkApps t l)
-  | value_stuck_fix f args (guarded : with_guarded_fix) :
-      All value args ->
-      isStuckFix f args ->
-      value (mkApps f args)
-  .
+   Lemma value_app f args : value_head #|args| f -> All value args -> value (mkApps f args).
+   Proof.
+     destruct args.
+     - intros [] hv; now constructor.
+     - intros vh av. eapply value_app_nonnil => //.
+   Qed.
 
-  Lemma value_values_ind : forall P : term -> Type,
-      (forall t, atom t -> P t) ->
-      (forall t l, value_head t -> All value l -> All P l -> P (mkApps t l)) ->
-      (forall f args (guarded : with_guarded_fix),
-          All value args ->
-          All P args ->
-          isStuckFix f args ->
-          P (mkApps f args)) ->
-      forall t : term, value t -> P t.
-  Proof.
-    intros P ? ? ?.
-    fix value_values_ind 2. destruct 1.
-    - apply X; auto.
-    - eapply X0; auto.
-      revert l a. fix aux 2. destruct 1. constructor; auto.
-      constructor. eauto. eauto.
-    - eapply X1; eauto.
-      clear i. revert args a. fix aux 2. destruct 1. constructor; auto.
-      constructor. now eapply value_values_ind. now apply aux.
-  Defined.
-
-  Lemma value_head_nApp {t} : value_head t -> ~~ isApp t.
-  Proof. destruct t; auto. Qed.
-  Hint Resolve value_head_nApp : core.
-
-  Lemma isStuckfix_nApp {t args} : isStuckFix t args -> ~~ isApp t.
-  Proof. destruct t; auto. Qed.
-  Hint Resolve isStuckfix_nApp : core.
-
-  Lemma atom_nApp {t} : atom t -> ~~ isApp t.
-  Proof. destruct t; auto. Qed.
-  Hint Resolve atom_nApp : core.
-
-  Lemma value_mkApps_inv t l :
-    ~~ isApp t ->
-    value (mkApps t l) ->
-    ((l = []) /\ atom t) + (value_head t × All value l) + (with_guarded_fix × isStuckFix t l × All value l).
-  Proof.
-    intros H H'. generalize_eqs H'. revert t H. induction H' using value_values_ind.
-    intros.
-    subst.
-    - now eapply atom_mkApps in H.
-    - intros * isapp appeq. move: (value_head_nApp H) => Ht.
-      apply mkApps_eq_inj in appeq; intuition subst; auto.
-    - intros * isapp appeq. move: (isStuckfix_nApp H) => Hf.
-      apply mkApps_eq_inj in appeq; intuition subst; auto.
-  Qed.
+   Lemma value_values_ind : forall P : term -> Type,
+       (forall t, atom t -> P t) ->
+       (forall f args, value_head #|args| f -> args <> [] -> All value args -> All P args -> P (mkApps f args)) ->
+       forall t : term, value t -> P t.
+   Proof.
+     intros P ??.
+     fix value_values_ind 2. destruct 1.
+     - apply X; auto.
+     - eapply X0; auto; tea.
+       clear v n. revert args a. fix aux 2. destruct 1. constructor; auto.
+       constructor. now eapply value_values_ind. now apply aux.
+   Defined.
+ 
+   Lemma value_head_nApp {nargs t} : value_head nargs t -> ~~ isApp t.
+   Proof. destruct 1; auto. Qed.
+   Hint Resolve value_head_nApp : core.
+ 
+   Lemma isStuckfix_nApp {t args} : isStuckFix t args -> ~~ isApp t.
+   Proof. destruct t; auto. Qed.
+   Hint Resolve isStuckfix_nApp : core.
+ 
+   Lemma atom_nApp {t} : atom t -> ~~ isApp t.
+   Proof. destruct t; auto. Qed.
+   Hint Resolve atom_nApp : core.
+ 
+   Lemma value_mkApps_inv t l :
+     ~~ isApp t ->
+     value (mkApps t l) ->
+     ((l = []) × atom t) + ([× l <> [], value_head #|l| t & All value l]).
+   Proof.
+     intros H H'. generalize_eq x (mkApps t l).
+     revert t H. induction H' using value_values_ind.
+     intros. subst.
+     - now eapply atom_mkApps in H.
+     - intros * isapp appeq. move: (value_head_nApp H) => Ht.
+       right. apply mkApps_eq_inj in appeq => //. intuition subst; auto => //.
+   Qed.
+   
+   Lemma value_mkApps_values t l :
+     value (mkApps t l) ->
+     ~~ isApp t ->
+     All value l.
+   Proof.
+     intros val not_app.
+     now apply value_mkApps_inv in val as [(-> & ?)|[]].
+   Qed.
+  
+   Lemma eval_to_value e e' : eval e e' -> value e'.
+   Proof.
+     intros ev. induction ev; simpl; intros; auto using value.
+ 
+     - change (tApp ?h ?a) with (mkApps h [a]).
+       rewrite -mkApps_app.
+       apply value_mkApps_inv in IHev1; [|easy].      
+       destruct IHev1 as [(-> & _)|[]].
+       + apply value_app; auto. len.
+         cbn in *. econstructor; tea.
+         destruct with_guarded_fix => //. cbn; auto.
+       + depelim v. rewrite e0 in e. noconf e.
+         eapply value_app; auto. econstructor; tea.
+         destruct with_guarded_fix => //.
+          len; lia. apply All_app_inv; auto.
+           
+     - apply value_mkApps_inv in IHev1; [|easy].      
+       destruct IHev1 as [(-> & _)|[]].
+       + cbn. eapply (value_app _ [a']); cbn; auto. econstructor; tea.
+       + rewrite -[tApp _ _](mkApps_app _ _ [a']).
+         eapply value_app. cbn; auto. econstructor; tea. cbn; len.
+         eapply All_app_inv; auto.
+ 
+     - destruct (mkApps_elim f' [a']).
+       eapply value_mkApps_inv in IHev1 => //.
+       destruct IHev1 as [?|[]]; intuition subst.
+       * rewrite a0.
+         simpl. rewrite a0 in i. simpl in *.
+         apply (value_app f0 [a']). 
+         destruct f0; simpl in * |- *; try congruence.
+         + rewrite !negb_or /= in i; rtoProp; intuition auto.
+         + rewrite !negb_or /= in i; rtoProp; intuition auto.
+         + destruct with_guarded_fix.
+          now cbn in i. now cbn in i.
+         + constructor.
+         + econstructor; auto.
+       * rewrite -[tApp _ _](mkApps_app _ (firstn n l) [a']).
+         eapply value_app; eauto with pcuic. 2:eapply All_app_inv; auto.
+         len.
+         rewrite isFixApp_mkApps isConstructApp_mkApps // in i.
+         rewrite !negb_or in i. rtoProp; intuition auto.
+         destruct with_guarded_fix eqn:gfix.
+         { destruct v; cbn in * => //. constructor. }
+        { destruct v; cbn in * => //; try now constructor.
+          now rewrite gfix in y. }
+   Qed.
+ 
+   Lemma value_head_spec n t :
+     value_head n t -> (~~ (isLambda t || isBox t)).
+   Proof.
+     destruct 1; simpl => //.
+   Qed.
+ 
+   Lemma value_head_final n t :
+     value_head n t -> eval t t.
+   Proof.
+     destruct 1.
+     - now constructor.
+     - now eapply eval_atom.
+     - now eapply eval_atom. 
+   Qed.
+ 
 
   (** The codomain of evaluation is only values: *)
   (*     It means no redex can remain at the head of an evaluated term. *)
 
-  Lemma value_head_spec t :
-    value_head t = (~~ (isLambda t || isFix t || isBox t)) && atom t.
+  Lemma value_head_spec' n t :
+    value_head n t -> (~~ (isLambda t || isBox t)) && atom t.
   Proof.
-    destruct t; intuition auto.
+    induction 1; cbn => //.
   Qed.
 
-  Lemma isFixApp_mkApps f args : ~~ isApp f -> isFixApp (mkApps f args) = isFixApp f.
-  Proof.
-    move=> Hf.
-    rewrite /isFixApp !decompose_app_mkApps // /=. now eapply negbTE in Hf.
-    change f with (mkApps f []) at 2.
-    rewrite !decompose_app_mkApps // /=. now eapply negbTE in Hf.
-  Qed.
-
-  Lemma eval_to_value e e' : eval e e' -> value e'.
-  Proof.
-    induction 1; simpl; auto using value.
-    - change (tApp ?h ?a) with (mkApps h [a]).
-      rewrite -mkApps_app.
-      apply value_mkApps_inv in IHeval1; [|easy].
-      destruct IHeval1 as [[(-> & _)|]|(stuck & vals)].
-      + cbn in *.
-        apply (value_stuck_fix _ [av]); [eauto|easy|].
-        cbn.
-        destruct (cunfold_fix mfix idx) as [(? & ?)|]; [|easy].
-        noconf e. destruct narg; auto. lia.
-      + easy.
-      + eapply value_stuck_fix;  [easy | now apply All_app_inv|].
-        unfold isStuckFix in *.
-        destruct (cunfold_fix mfix idx) as [(? & ?)|]; [|easy].
-        noconf e. rewrite app_length; simpl.
-        eapply Nat.leb_le. lia.
-
-    - destruct (mkApps_elim f' [a']).
-      eapply value_mkApps_inv in IHeval1 => //.
-      destruct IHeval1; intuition subst.
-      * rewrite -> H1 in *.
-        simpl in *.
-        apply (value_app f0 [a']). destruct with_guarded_fix;
-        destruct f0; simpl in * |- *; try congruence;
-           constructor; auto. constructor; eauto. 
-      * rewrite -[tApp _ _](mkApps_app _ (firstn n l) [a']).
-        constructor 2; auto. eapply All_app_inv; auto.
-      * rewrite -[tApp _ _](mkApps_app _ (firstn n l) [a']).
-        erewrite isFixApp_mkApps in i => //.
-        destruct f0; simpl in *; try congruence.
-        rewrite /isFixApp in i. simpl in i.
-        rewrite a0 in i.
-        rewrite orb_true_r orb_true_l in i. easy.         
-  Qed.
 
   Lemma closed_fix_substl_subst_eq {mfix idx d} : 
     closed (tFix mfix idx) ->
@@ -436,44 +485,33 @@ Section Wcbv.
     induction 1; constructor; auto.
   Qed.
 
-  Lemma value_head_spec_impl t :
-    implb (value_head t) (~~ (isLambda t || (if with_guarded_fix then isFixApp t else isFix t) || isBox t)).
+  (* Lemma value_head_spec_impl t :
+    value_head t) (~~ (isLambda t || (if with_guarded_fix then isFixApp t else isFix t) || isBox t)).
   Proof.
     destruct with_guarded_fix;
     destruct t; simpl; intuition auto; eapply implyb.
-  Qed.
+  Qed. *)
 
   Derive Signature for Forall.
 
-  Lemma eval_stuck_fix args argsv mfix idx :
+  Lemma eval_stuck_Fix {f mfix idx args args'} :
     with_guarded_fix ->
-    All2 eval args argsv ->
-    isStuckFix (tFix mfix idx) argsv ->
-    eval (mkApps (tFix mfix idx) args) (mkApps (tFix mfix idx) argsv).
+    eval f (tFix mfix idx) ->
+    All2 eval args args' ->
+    isStuckFix (tFix mfix idx) args ->
+    eval (mkApps f args) (mkApps (tFix mfix idx) args').
   Proof.
-    intros guarded.
-    revert argsv.
-    induction args as [|a args IH] using MCList.rev_ind;
-    intros argsv all stuck.
-    - apply All2_length in all.
-      destruct argsv; [|easy].
-      now apply eval_atom.
-    - destruct argsv as [|? ? _] using MCList.rev_ind;
-        [apply All2_length in all; rewrite app_length in all; now cbn in *|].
-      apply All2_app_r in all as (all & ev_a).
-      rewrite !mkApps_app.
-      cbn in *.
-      destruct (cunfold_fix mfix idx) as [(? & ?)|] eqn:cuf; [|easy].
-      eapply eval_fix_value.
-      + easy.
-      + eapply IH; [easy|].
-        destruct (cunfold_fix mfix idx) as [(? & ?)|]; [|easy].
-        rewrite app_length /= in stuck.
-        eapply Nat.leb_le in stuck. eapply Nat.leb_le. lia.
-      + easy.
-      + easy.
-      + rewrite app_length /= in stuck.
-        eapply Nat.leb_le in stuck; lia.
+    intros wgf evf hargs. revert args' hargs.
+    induction args using rev_ind; intros args' evargs.
+    - depelim evargs. cbn; auto.
+    - eapply All2_app_inv_l in evargs as [r1 [r2 [-> [evl evr]]]].
+      depelim evr. depelim evr.
+      rewrite !mkApps_app /=.
+      destruct cunfold_fix as [[rarg fn]|] eqn:eqc => //.
+      len; cbn. move/Nat.leb_le => hrarg.
+      eapply eval_fix_value. auto. 
+      eapply IHargs => //. unfold isStuckFix. rewrite eqc. apply Nat.leb_le; lia. auto. tea.
+      rewrite -(All2_length evl). lia.
   Qed.
 
   Lemma stuck_fix_value_inv argsv mfix idx narg fn :
@@ -487,8 +525,9 @@ Section Wcbv.
     unfold atom in H. destruct argsv using rev_case => //.
     split; auto. simpl. simpl in H. rewrite H0 //.
     rewrite mkApps_app /= in H. depelim H.
-    solve_discr => //.
-    solve_discr.
+    solve_discr => //. depelim H. rewrite e.
+    intros [= <- <-]. destruct with_guarded_fix => //. split => //.
+    unfold isStuckFix. rewrite e. now apply Nat.leb_le.
   Qed.
     
   Lemma stuck_fix_value_args argsv mfix idx narg fn :
@@ -503,35 +542,92 @@ Section Wcbv.
     now eapply Nat.leb_le in i.
   Qed.
 
+  Lemma eval_mkApps_Construct ind c mdecl idecl cdecl f args args' :
+    lookup_constructor Σ ind c = Some (mdecl, idecl, cdecl) ->
+    eval f (tConstruct ind c) ->
+    #|args| <= cstr_arity mdecl cdecl ->
+    All2 eval args args' ->
+    eval (mkApps f args) (mkApps (tConstruct ind c) args').
+  Proof.
+    intros hdecl evf hargs. revert args'.
+    induction args using rev_ind; intros args' evargs.
+    - depelim evargs. now cbn.
+    - eapply All2_app_inv_l in evargs as [r1 [r2 [-> [evl evr]]]].
+      depelim evr. depelim evr.
+      rewrite mkApps_app /=. len in hargs. cbn in hargs.
+      rewrite mkApps_app.
+      eapply eval_construct; tea.
+      eapply IHargs => //. lia.
+      rewrite -(All2_length evl). lia.
+  Qed.
+
+  Lemma nisLambda_mkApps f args : ~~ isLambda f -> ~~ isLambda (mkApps f args).
+  Proof. destruct args using rev_case => //. rewrite mkApps_app /= //. Qed.
+  Lemma nisFix_mkApps f args : ~~ isFix f -> ~~ isFix (mkApps f args).
+  Proof. destruct args using rev_case => //. rewrite mkApps_app /= //. Qed.
+  Lemma nisBox_mkApps f args : ~~ isBox f -> ~~ isBox (mkApps f args).
+  Proof. destruct args using rev_case => //. rewrite mkApps_app /= //. Qed.
+
+  Lemma eval_mkApps_CoFix f mfix idx args args' :
+    eval f (tCoFix mfix idx) ->
+    All2 eval args args' ->
+    eval (mkApps f args) (mkApps (tCoFix mfix idx) args').
+  Proof.
+    intros evf hargs. revert args' hargs.
+    induction args using rev_ind; intros args' evargs.
+    - depelim evargs. cbn; auto.
+    - eapply All2_app_inv_l in evargs as [r1 [r2 [-> [evl evr]]]].
+      depelim evr. depelim evr.
+      rewrite !mkApps_app /=.
+      eapply eval_app_cong; tea. 
+      eapply IHargs => //.
+      rewrite isFixApp_mkApps // /= isConstructApp_mkApps // !negb_or. rtoProp; intuition auto.
+      apply nisLambda_mkApps => //.
+      destruct with_guarded_fix => //; eapply nisFix_mkApps => //.
+      apply nisBox_mkApps => //.
+  Qed.
+
+  Lemma eval_mkApps_tBox f args args' :
+    eval f tBox ->
+    All2 eval args args' ->
+    eval (mkApps f args) tBox.
+  Proof.
+    intros evf hargs. revert args' hargs.
+    induction args using rev_ind; intros args' evargs.
+    - depelim evargs. cbn; auto.
+    - eapply All2_app_inv_l in evargs as [r1 [r2 [-> [evl evr]]]].
+      depelim evr. depelim evr.
+      rewrite !mkApps_app /=.
+      eapply eval_box; tea.
+      eapply IHargs => //. eapply evl.
+  Qed.
+
+  Lemma eval_mkApps_cong f f' l l' :
+    eval f f' ->
+    value_head #|l| f' ->
+    All2 eval l l' ->
+    eval (mkApps f l) (mkApps f' l').
+  Proof.
+    revert l'. induction l using rev_ind; intros l' evf vf' evl.
+    depelim evl. eapply evf.
+    eapply All2_app_inv_l in evl as (?&?&?&?&?).
+    intuition auto. subst. depelim a0. depelim a0.
+    - destruct vf'.
+      * eapply eval_mkApps_Construct; tea. eapply All2_app; auto.
+      * eapply eval_mkApps_CoFix; auto. eapply All2_app; auto.
+      * destruct with_guarded_fix eqn:wgf => //.
+        eapply eval_stuck_Fix; tea. eapply All2_app; auto.
+        unfold isStuckFix; rewrite e0. now apply Nat.leb_le.
+  Qed.
+
   Lemma value_final e : value e -> eval e e.
   Proof.
     induction 1 using value_values_ind; simpl; auto using value.
-    - apply All_All2_refl in X0 as H2.
-      move/implyP: (value_head_spec_impl t).
-      move/(_ H) => Ht.
-      induction l using rev_ind. simpl.
-      destruct t; try discriminate.
-      * repeat constructor.
-      * repeat constructor.
-      * rewrite mkApps_app.
-        eapply All_app in X as [Hl Hx]. depelim Hx.
-        eapply All_app in X0 as [Hl' Hx']. depelim Hx'.
-        eapply All2_app_inv_r in H2 as [Hl'' [Hx'' [? [? ?]]]].
-        depelim a0.
-        eapply eval_app_cong; auto.
-        eapply IHl; auto.
-        now eapply All_All2.
-        destruct l using rev_ind; auto.
-        eapply value_head_nApp in H.
-        rewrite isFixApp_mkApps => //.
-        rewrite mkApps_app; simpl.
-        destruct with_guarded_fix => //.
-        destruct t => //.
-    - destruct f; try discriminate.
-      apply All_All2_refl in X0.
-      eapply eval_stuck_fix; eauto.
+    assert (All2 eval args args).
+    { clear -X0; induction X0; constructor; auto. }
+    eapply eval_mkApps_cong => //. now eapply value_head_final. 
   Qed.
-
+  
   Set Equations With UIP.
 
   Unset SsrRewrite.
@@ -559,16 +655,15 @@ Section Wcbv.
     - depelim ev'; go.
     - depelim ev'; try go.
       + specialize (IHev1 _ ev'1); noconf IHev1.
-        apply (f_equal pr1) in IHev1 as apps_eq; cbn in *.
+        apply (f_equal pr1) in IHev1 as apps_eq. cbn in apps_eq.
         apply mkApps_eq_inj in apps_eq as (eq1 & eq2); try easy.
-        noconf eq1.
-        noconf eq2.
+        noconf eq1. noconf eq2.
         noconf IHev1.
-        pose proof e0. rewrite e3 in H. noconf H.
-        rewrite (uip e0 e3).
-        rewrite (uip e e2).
+        pose proof e0. rewrite e4 in H. noconf H.
+        pose proof e as e'. rewrite e3 in e'. noconf e'.
+        rewrite (uip e e3), (uip e0 e4), (uip e1 e5), (uip e2 e6).
         specialize (IHev2 _ ev'2); noconf IHev2.
-        now rewrite (uip e1 e4).
+        reflexivity.
     - depelim ev'; try go.
       + subst.
         noconf e2.
@@ -667,31 +762,42 @@ Section Wcbv.
     - depelim ev'; try go.
       specialize (IHev1 _ ev'1).
       pose proof (mkApps_eq_inj (f_equal pr1 IHev1) eq_refl eq_refl) as (? & <-).
-      noconf H.
-      noconf IHev1.
-      rewrite (uip e e0).
+      noconf H. noconf IHev1.
+      pose proof e as e'. rewrite e2 in e'; noconf e'.
+      rewrite (uip e e2), (uip e0 e3).
+      pose proof e4 as e4'. rewrite e1 in e4'; noconf e4'.
+      rewrite (uip e1 e4).
       now specialize (IHev2 _ ev'2); noconf IHev2.
     - depelim ev'; try go.
       specialize (IHev _ ev'). noconf IHev.
       rewrite (uip e e0).
       now rewrite (uip i0 i2).
     - depelim ev'; try go.
-      + specialize (IHev1 _ ev'1); noconf IHev1.
-        exfalso; destruct with_guarded_fix; cbn in *; easy.
-      + specialize (IHev1 _ ev'1); noconf IHev1.
-        exfalso.
-        rewrite isFixApp_mkApps in i; try easy.
-        cbn in *.
-        destruct with_guarded_fix; try easy.
-        now rewrite Bool.orb_true_r in i.
-      + specialize (IHev1 _ ev'1); noconf IHev1.
-        exfalso.
-        rewrite isFixApp_mkApps in i; try easy.
-        cbn in *.
-        destruct with_guarded_fix; try easy.
-        now rewrite Bool.orb_true_r in i.
-      + specialize (IHev1 _ ev'1); noconf IHev1.
-        exfalso. rewrite unguarded in i. easy.
+      + move: (IHev1 _ ev'1).
+        eapply DepElim.simplification_sigma1 => heq IHev1'.
+        apply mkApps_eq_inj in heq as H'; auto.
+        destruct H' as (H' & <-). noconf H'.
+        noconf IHev1'.
+        pose proof e as e'. rewrite e0 in e'; noconf e'.
+        specialize (IHev2 _ ev'2). noconf IHev2.
+        now rewrite (uip e e0), (PCUICWcbvEval.le_irrel _ _ l l0).
+      + specialize (IHev1 _ ev'1). noconf IHev1.
+        exfalso. rewrite isConstructApp_mkApps in i.
+        cbn in i. rewrite !negb_or in i. rtoProp; intuition auto.
+    - depelim ev'; try go.
+      + exfalso. rewrite !negb_or in i. specialize (IHev1 _ ev'1); noconf IHev1.
+        cbn in i. rtoProp; intuition auto.
+      + exfalso. rewrite !negb_or in i. specialize (IHev1 _ ev'1); noconf IHev1.
+        cbn in i. rewrite guarded in i. rtoProp; intuition auto.
+        rewrite isFixApp_mkApps in H2 => //.
+      + exfalso. rewrite !negb_or in i. specialize (IHev1 _ ev'1); noconf IHev1.
+        cbn in i. rewrite guarded in i. rtoProp; intuition auto.
+        rewrite isFixApp_mkApps in H2 => //.
+      + exfalso. rewrite !negb_or in i. specialize (IHev1 _ ev'1); noconf IHev1.
+        cbn in i. rewrite unguarded in i. now cbn in i.
+      + exfalso. rewrite !negb_or in i. specialize (IHev1 _ ev'1); noconf IHev1.
+        cbn in i. rtoProp; intuition auto.
+        now rewrite isConstructApp_mkApps in H0.
       + specialize (IHev1 _ ev'1); noconf IHev1.
         specialize (IHev2 _ ev'2); noconf IHev2.
         now assert (i0 = i) as -> by now apply uip.
@@ -758,6 +864,10 @@ Section Wcbv.
         exists f'; split => //.
         rewrite mkApps_app.
         eapply eval_fix'; eauto.
+      + specialize (IHargs _ _ ev1) as [f' [evf' ev]].
+        exists f'; split => //.
+        rewrite mkApps_app.
+        eapply eval_construct; eauto.
       + specialize (IHargs _ _ ev1) as [f'' [evf' ev]].
         exists f''; split => //.
         rewrite mkApps_app.
@@ -821,12 +931,15 @@ Arguments eval_unique {_ _ _ _}.
 Section WcbvEnv.
   Context {wfl : WcbvFlags} {efl : EEnvFlags}.
 
+
+
   Lemma weakening_eval_env {Σ Σ'} : 
     wf_glob Σ' -> extends Σ Σ' ->
     forall v t, eval Σ v t -> eval Σ' v t.
   Proof.
     intros wf ex t v ev.
-    induction ev; try solve [econstructor; eauto using (extends_is_propositional wf ex)].
+    induction ev; try solve [econstructor; 
+      eauto using (extends_lookup_constructor wf ex), (extends_constructor_isprop_pars_decl wf ex), (extends_is_propositional wf ex)].
     econstructor; eauto.
     red in isdecl |- *. eauto using extends_lookup.
   Qed.
@@ -862,6 +975,13 @@ Proof.
     depelim ev; try solve_discr.
     destruct (IHargs _ ev1) as [? []]. solve_discr.
     all:try specialize (IHargs _ ev1) as [? []]; try solve_discr.
+    noconf H.
+    * rewrite -{1}[tApp _ _](mkApps_app _ _ [a']). eexists. split => //.
+      eapply All2_app; eauto.
+      eapply All2_impl; tea; cbv beta; intros ? ? [ev hev].
+      exists ev. cbn. lia.
+      constructor; auto. exists ev2.
+      cbn. lia.
     * subst f'. 
       exists (x0 ++ [a'])%list.
       rewrite mkApps_app /= //.
@@ -871,7 +991,7 @@ Proof.
     * now cbn in i.
 Qed.
 
-Lemma eval_mkApps_Construct {fl : WcbvFlags} Σ kn c args args' : 
+(* Lemma eval_mkApps_Construct' {fl : WcbvFlags} Σ kn c args args' : 
   All2 (eval Σ) args args' ->
   eval Σ (mkApps (tConstruct kn c) args) (mkApps (tConstruct kn c) args').
 Proof.
@@ -885,7 +1005,7 @@ Proof.
     destruct args' using rev_ind; try now rewrite ?mkApps_app; cbn; destruct with_guarded_fix; eauto.
     cbn. rewrite isFixApp_mkApps; eauto.
     cbn. try now rewrite ?mkApps_app; cbn; destruct with_guarded_fix; eauto.
-Qed.
+Qed. *)
 
 Require Import Utf8.
 From MetaCoq.Template Require Import BasicAst.
@@ -992,8 +1112,7 @@ Proof.
     move: IHev1; rewrite closedn_mkApps => /andP[] _ clargs.
     apply IHev2. rewrite /iota_red.
     eapply closed_substl. now rewrite forallb_rev forallb_skipn.
-    len.
-    rewrite e1. eapply nth_error_forallb in Hc'; tea.
+    len. rewrite e2. eapply nth_error_forallb in Hc'; tea.
     now rewrite Nat.add_0_r in Hc'.
   - subst brs. cbn in Hc'. rewrite andb_true_r in Hc'.
     eapply IHev2. eapply closed_substl.
@@ -1028,9 +1147,10 @@ Proof.
   - have := (IHev1 Hc).
     rewrite closedn_mkApps /= => clargs.
     eapply IHev2; eauto.
-    rewrite nth_nth_error.
-    destruct nth_error eqn:hnth => //.
     eapply nth_error_forallb in clargs; tea.
+  - have := (IHev1 Hc).
+    rewrite closedn_mkApps /= => clargs.
+    rewrite clargs IHev2 //.
   - rtoProp; intuition auto.
 Qed.
 
@@ -1041,7 +1161,13 @@ Ltac forward_keep H :=
     assert (H' : X) ; [|specialize (H H')]
   end.
 
-Lemma eval_wellformed (efl := all_env_flags) {wfl : WcbvFlags} Σ : 
+Definition mk_env_flags has_ax has_pars tfl :=  
+  {| has_axioms := has_ax;
+     has_cstr_params := has_pars;
+     term_switches := tfl |}.
+    
+Lemma eval_wellformed has_ax has_pars (efl := mk_env_flags has_ax has_pars all_term_flags)
+  {wfl : WcbvFlags} Σ : 
   wf_glob Σ ->
   forall t u, wellformed Σ 0 t -> eval Σ t u -> wellformed Σ 0 u.
 Proof.
@@ -1050,7 +1176,7 @@ Proof.
     (move/andP=> [/andP[Hc Hc'] Hc''] || move/andP=> [Hc Hc'] || move=>Hc); auto.
   all:eauto using wellformed_csubst.
   - specialize (IHev1 Hc').
-    move: IHev1; rewrite wellformed_mkApps // => /andP[] wfc wfargs.
+    move: IHev1. rewrite wellformed_mkApps // => /andP[] wfc wfargs.
     apply IHev2.
     eapply wellformed_iota_red_brs; tea => //.
   - subst brs. cbn in Hc''. rewrite andb_true_r in Hc''.
@@ -1081,10 +1207,11 @@ Proof.
   - have := (IHev1 Hc').
     rewrite wellformed_mkApps // /= => clargs.
     eapply IHev2; eauto.
-    rewrite nth_nth_error.
-    destruct nth_error eqn:hnth => //.
     move/andP: clargs => [wfc wfargs].
     eapply nth_error_forallb in wfargs; tea.
+  - have := IHev1 Hc.
+    rewrite !wellformed_mkApps // /=.
+    now move/andP => [] -> -> /=.
   - rtoProp; intuition auto.
 Qed.
 
@@ -1107,7 +1234,8 @@ Local Hint Rewrite @remove_last_length : len.
 Lemma eval_mkApps_tFix_inv_size {wfl : WcbvFlags} Σ mfix idx args v :
   with_guarded_fix ->
   forall Heval : eval Σ (mkApps (tFix mfix idx) args) v,
-  (∑ args', All2 (fun a a' => ∑ H : eval Σ a a', eval_depth H < eval_depth Heval) args args' × v = mkApps (tFix mfix idx) (args')) +
+  (∑ args', All2 (fun a a' => ∑ H : eval Σ a a', eval_depth H < eval_depth Heval) args args' ×
+     v = mkApps (tFix mfix idx) (args')) +
   (∑ n b, args <> nil /\ cunfold_fix mfix idx = Some (n, b) /\ n < #|args|).
 Proof.
  revert v.
@@ -1117,20 +1245,20 @@ Proof.
    cbn in *.
    depelim ev.
   
-   all: try(specialize (IHargs) with (Heval := ev1); destruct IHargs as [(args' & ? & Heq) | (? & ? & ? & ? & ?)];eauto; rewrite ?Heq; try solve_discr; try congruence;
+   all: try(specialize (IHargs) with (Heval := ev1); 
+    destruct IHargs as [(args' & ? & Heq) | (? & ? & ? & ? & ?)];eauto; 
+      rewrite ?Heq; try solve_discr; try congruence; try noconf H;
      len; rewrite ?Heq; rewrite Nat.add_comm; eauto 9).
-   * right. repeat eexists. destruct args; cbn; congruence. eauto. lia.
-   * right. repeat eexists. destruct args; cbn; congruence. eauto. lia.
-   * invs H. eapply All2_length in a. right. repeat eexists. destruct args; cbn; congruence. eauto. lia.
-   * right. repeat eexists. destruct args; cbn; congruence. eauto. lia.
-   * invs H. left. eexists. split. sq. eapply All2_app. solve_all. destruct H. unshelve eexists. eauto. cbn. lia.
+   * right. repeat eexists. destruct args; cbn; congruence. eauto.
+     rewrite (All2_length a); lia.
+   * left. eexists. split. sq. eapply All2_app. solve_all. destruct H. unshelve eexists. eauto. cbn. lia.
      econstructor. 2: econstructor.
      unshelve eexists. eauto. lia.
      now rewrite !mkApps_app.
-   * right. repeat eexists. destruct args; cbn; congruence. eauto. lia.
-   * subst. sq.  rewrite wg in i. rewrite isFixApp_mkApps in i => //. cbn in i. destruct EAst.isLambda; easy.
-   * right. repeat eexists. destruct args; cbn; congruence. eauto. lia.
-   * inv i.
+   * subst f'. rewrite wg in i.
+     rewrite isFixApp_mkApps /= /isFixApp /= in i.
+     rewrite !negb_or in i; rtoProp; intuition auto. now cbn in H2.
+   * now cbn in i.
 Qed.
 
 Lemma size_final {wfl : WcbvFlags} Σ t v :
@@ -1143,6 +1271,8 @@ Proof.
   all: try now unshelve eexists; eauto; cbn; lia.
   - unshelve eexists. repeat econstructor. cbn; lia.
   - unshelve eexists; eauto. eapply eval_fix_value; eauto. eapply IHHe1. eapply IHHe2. cbn. destruct IHHe1, IHHe2. lia.
+  - unshelve eexists. eapply eval_construct; eauto.
+    eapply IHHe1. eapply IHHe2. cbn. destruct IHHe1, IHHe2. cbn. lia.
   - unshelve eexists. eapply eval_app_cong; eauto. eapply IHHe1. eapply IHHe2. cbn. destruct IHHe1, IHHe2. lia.
 Qed.
 
@@ -1194,6 +1324,19 @@ Proof.
      3:tea. cbn in *; lia.
      cbn. generalize (mkApps_app (tApp fn_ aval) argsv_ [x]). generalize (EAst.mkApps (tApp fn_ aval) (argsv_ ++ [x])). intros. subst. cbn.
      cbn in *. lia.
+   * subst. exists a, aval, (args' ++ [x]), (argsv_ ++ [a']).
+     split => //. split.
+     { eapply All2_app.
+      - eapply All2_impl; tea; cbv beta.
+        intros ?? [eq|[H IH]]; intuition auto. right; exists H. cbn. clear -IH. cbn in *. lia.
+      - constructor; auto.
+        right; exists ev2. cbn; lia. }
+    exists n, fn_. split => //.
+    exists Heva; cbn. split => //. cbn in *; lia.
+    rewrite mkApps_app /=.
+    unshelve eexists. eapply eval_construct; tea.
+    exact (size_final _ _ _ ev2).π1.
+    cbn. destruct size_final; cbn. cbn in *. lia.
    * subst. cbn in i. exfalso. destruct with_guarded_fix; easy.
    * subst.  cbn. eexists _, _, _, (argsv_ ++ [_])%list. repeat eexists. 2: eauto.
      eapply All2_app.
@@ -1205,15 +1348,18 @@ Proof.
    * subst. cbn. invs i.
 Qed.
 
-Lemma eval_construct  {fl : WcbvFlags} Σ kn c args e : 
-  eval Σ (mkApps (tConstruct kn c) args) e -> ∑ args', (e = mkApps (tConstruct kn c) args') × All2 (eval Σ) args args'.
+Lemma eval_construct' {fl : WcbvFlags} Σ kn c args e : 
+  eval Σ (mkApps (tConstruct kn c) args) e -> 
+  ∑ args', (e = mkApps (tConstruct kn c) args') × All2 (eval Σ) args args'.
 Proof.
   revert e; induction args using rev_ind; intros e.
   - intros ev. depelim ev. exists []=> //.
   - intros ev. rewrite mkApps_app /= in ev.
     depelim ev; try solve_discr.
     destruct (IHargs _ ev1) as [? []]. solve_discr.
-    all:try specialize (IHargs _ ev1) as [? []]; try solve_discr.
+    all:try specialize (IHargs _ ev1) as [? []]; try solve_discr; try noconf H.
+    * exists (x0 ++ [a']). split => //.
+      rewrite mkApps_app /= //. eapply All2_app; eauto.
     * subst f'. 
       exists (x0 ++ [a'])%list.
       rewrite mkApps_app /= //.
